coq/LLVMGen/tmp_aux_Vellvm.v
@@ -44,6 +44,8 @@ Import IS.
 Import M.
 
 
+Section InterpreterCFG.
+
 (**
    Partial interpretations of the trees produced by the
    denotation of cfg. They differ from the ones of Vellvm programs by
@@ -153,6 +155,9 @@ Proof.
   rewrite INT.interp_intrinsics_ret, interp_global_ret, interp_local_ret, interp_memory_ret; reflexivity.
 Qed.
 
+End InterpreterCFG.
+
+Section Denotation.
 Import CatNotations.
 
 Lemma denote_bks_nil: forall s, D.denote_bks [] s ≈ ret (inl s).
@@ -167,6 +172,68 @@ Proof.
   repeat (cbn; (rewrite bind_bind || rewrite bind_ret_l)).
   reflexivity.
 Qed.
+
+  From Vellvm Require Import Util.
+  Require Import State.
+
+Instance eutt_interp_cfg_to_L3 (defs: intrinsic_definitions) {T}:
+  Proper (eutt Logic.eq ==> Logic.eq ==> Logic.eq ==> Logic.eq ==> eutt Logic.eq) (@interp_cfg_to_L3 T defs).
+Proof.
+  repeat intro.
+  unfold interp_cfg_to_L3, Util.runState.
+  subst; rewrite H.
+  reflexivity.
+Qed.
+
+(* TODOYZ: This is weird, I need to import again this file for the rewriting to work.
+   A bit unsure as to why this happen, but somehow some subsequent import breaks it.
+ *)
+Require Import ITree.Eq.Eq.
+
+Lemma denote_bks_singleton :
+  forall (b : LLVMAst.block dtyp) (bid : block_id) (nextblock : block_id),
+    blk_id b = bid ->
+    (snd (blk_term b)) = (TERM_Br_1 nextblock) ->
+    (blk_id b) <> nextblock ->
+    eutt (Logic.eq) (D.denote_bks [b] bid) (D.denote_block b).
+Proof.
+  intros b bid nextblock Heqid Heqterm Hneq.
+  cbn.
+  rewrite bind_ret_l.
+  rewrite KTreeFacts.unfold_iter_ktree.
+  cbn.
+  destruct (Eqv.eqv_dec_p (blk_id b) bid) eqn:Heq'; try contradiction.
+  repeat rewrite bind_bind.
+  rewrite Heqterm.
+  cbn.
+  setoid_rewrite translate_ret.
+  setoid_rewrite bind_ret_l.
+  destruct (Eqv.eqv_dec_p (blk_id b) nextblock); try contradiction.
+  repeat setoid_rewrite bind_ret_l. unfold Datatypes.id.
+  reflexivity.
+Qed.
+
+Lemma denote_code_app :
+  forall a b,
+    D.denote_code (a ++ b) ≈ ITree.bind (D.denote_code a) (fun _ => D.denote_code b).
+Proof.
+  induction a; intros b.
+  - cbn. rewrite bind_ret_l.
+    reflexivity.
+  - cbn. rewrite bind_bind. setoid_rewrite IHa.
+    reflexivity.
+Qed.
+
+Lemma denote_code_cons :
+  forall a l,
+    D.denote_code (a::l) ≈ ITree.bind (D.denote_instr a) (fun _ => D.denote_code l).
+Proof.
+  cbn; reflexivity.
+Qed.
+
+End Denotation.
+
+Section NormalizeTypes.
 
 Lemma normalize_types_block_bid :
   forall (env : list (ident * typ)) (b: LLVMAst.block typ),
@@ -186,6 +253,50 @@ Proof.
   reflexivity.
 Qed.
 
+Definition normalize_types_blocks (env: list _) (bks: list (LLVMAst.block typ))
+  : list (LLVMAst.block DynamicTypes.dtyp) :=
+  List.map
+    (TransformTypes.fmap_block _ _ (TypeUtil.normalize_type_dtyp env)) bks.
+
+End NormalizeTypes.
+
+Section MemoryModel.
+
+  Definition get_logical_block (mem: M.memory) (ptr: A.addr): option M.logical_block :=
+    let '(b,a) := ptr in
+    M.lookup_logical b mem.
+
+End MemoryModel.
+
+Section ValuePred.
+  Import Integers.
+  Import BinInt.
+
+  Definition int64_dvalue_rel (n : Int64.int) (dv : dvalue) : Prop :=
+    match dv with
+    | DVALUE_I64 i => BinInt.Z.eq (Int64.intval n) (unsigned i)
+    | _ => False
+    end.
+
+  Definition nat_dvalue_rel (n : nat) (dv : dvalue) : Prop :=
+    match dv with
+    | DVALUE_I64 i => Z.eq (Z.of_nat n) (unsigned i)
+    | _ => False
+    end.
+
+  Definition int64_concrete_uvalue_rel (n : Int64.int) (uv : uvalue) : Prop :=
+    match uvalue_to_dvalue uv with
+    | inr dv => int64_dvalue_rel n dv
+    | _ => False
+    end.
+
+  Definition nat_concrete_uvalue_rel (n : nat) (uv : uvalue) : Prop :=
+    match uvalue_to_dvalue uv with
+    | inr dv => nat_dvalue_rel n dv
+    | _ => False
+    end.
+
+End ValuePred.
 
 (* Instance eutt_interp_cfg_to_L3 (defs: intrinsic_definitions) {T}: *)
 (*   Proper (eutt Logic.eq ==> Logic.eq ==> Logic.eq ==> Logic.eq ==> eutt Logic.eq) (@interp_cfg_to_L3 T defs). *)
